

# Quiz 4

Nixx Vorboncoer  
12/3/25

[1]  $f_s = 44100$   $(s)$   $H_z = 500$   $\theta(\omega)^L = 0.5$

$L =$   $\alpha =$  delay total =  $f_s \delta = L + 0.5 + \delta$

~~$y_t = x_t \cdot R^L x_{t-L}$~~   $0 \leq \delta \leq 1$

$88.2 = L + 0.5 + \delta$

$87.7 = L + \delta \rightarrow L = 87, \delta = 0.7$  (d)

[2] Comb:  $[-6, 24]$  dB  $dB = 20 \log_{10}(Hz)$

$\Delta = 30$  dB

$30 = 20 \log_{10}(Hz)$

$1.5 = \log_{10}(Hz)$

$10^{1.5} = Hz = 31.62 \approx 32$  (a)

[3]  $x_t = \frac{1}{2}(x_t + x_{t+1})$   $H(z) = \frac{1}{2} + \frac{1}{2}z^{-1}$   $H(\omega) = \frac{1}{2} + \frac{1}{2}e^{-j\omega}$

$H(z) = \frac{1}{2}(1 + z^{-1})$   $|H(\omega)| = \frac{1}{2} + \frac{1}{2}(\cos(\omega) - j \sin(\omega))$

$H(\omega) = \frac{1}{2}(1 + e^{-j\omega}) = \frac{1}{2}e^{-j\omega/2}(e^{j\omega/2} + e^{-j\omega/2})$   $\theta(\omega) = -\omega/2$

$(\cos(\omega/2) + j \sin(\omega/2)) + (\cos(\omega/2) - j \sin(\omega/2))$   
 $\frac{1}{2}e^{-j\omega/2}(2 \cos(\omega/2)) = \cos(\omega/2)e^{-j\omega/2}$

$H(\omega) = e^{-j\omega/2} \cos(\omega/2)$   $\theta(\omega) = -\omega/2$  Linear phase

$|H(\omega)| = [\cos(\omega/2) \cdot \cos(\omega/2)]^{1/2}$   $|\cos(\omega/2) - j \sin(\omega/2)| =$   
 $= [2 \cos^2(\omega/2)]^{1/2}$   $[\cos^2(\omega/2) + \sin^2(\omega/2)]^{1/2}$   
 $= \cos(\omega/2)$   $\sqrt{1} = 1$

$|H(\omega)| = |1 \cdot \cos(\omega/2)| = \cos(\omega/2) \therefore$  (d)

$$[4] Y_t = aX_t + X_{t-1} - aY_{t-1}$$

$$Y_t + aY_{t-1} = aX_t + X_{t-1}$$

$$H(z) = \frac{a+z^{-1}}{1+az^{-1}}$$

$$Y(z)(1+az^{-1}) = X(z)(a+z^{-1}) \Rightarrow \frac{Y(z)}{X(z)} = \frac{a+z^{-1}}{1+az^{-1}}$$

Pole:

$$0 = 1+az^{-1} \Rightarrow -1 > a \frac{1}{z} = -\frac{1}{a} = \frac{1}{z} \Rightarrow -a = z$$

1 Pole

$$H(\omega) = \frac{a + e^{-j\omega}}{1 + ae^{-j\omega}} \quad |H(\omega)| = \frac{|a + e^{-j\omega}|^2}{|1 + ae^{-j\omega}|^2}$$

$$|a + e^{-j\omega}|^2 = [a^2 + (\cos(\omega) + j\sin(\omega))]^2$$

$$= a^2 + 2a\cos(\omega) + \cos^2(\omega) + \sin^2(\omega) = a^2 + 2a\cos(\omega) + 1$$

$$|1 + ae^{-j\omega}|^2 = [1 + a\cos(\omega)]^2 + [a\sin(\omega)]^2$$

$$= 1 + 2a\cos(\omega) + a^2\cos^2(\omega) + a^2\sin^2(\omega) = 1 + 2a\cos(\omega) + a^2(\cos^2(\omega) + \sin^2(\omega)) = 1 + 2a\cos(\omega) + a^2(1)$$

$$|H(\omega)| = \frac{a^2 + 2a\cos(\omega) + 1}{a^2 + 2a\cos(\omega) + 1} = 1$$

$$H(\omega) = \frac{a + \cos(\omega) - j\sin(\omega)}{1 + a[\cos(\omega) - j\sin(\omega)]}$$

$$\theta(\omega)_N = \tan^{-1} \frac{-\sin(\omega)}{a + \cos(\omega)}$$

$$\theta(\omega)_0 = \tan^{-1} \frac{-a\sin(\omega)}{1 + a\cos(\omega)}$$

Phase control on a ✓

d



$$[5] \textcircled{a} H(z) = \frac{\frac{1}{2}z + 1}{z + \frac{1}{2}}$$

$$\frac{Y(z)}{X(z)} = \frac{\frac{1}{2}z + 1}{z + \frac{1}{2}}$$

$$\text{allpass: } H(z) = \frac{a + z}{1 + az}$$

$$|H(\omega)| = 1$$

$$X(z)(z + \frac{1}{2}) = Y(z)(\frac{1}{2}z + 1)$$

$$Y(z)(\frac{1}{2}z^{-1} + 1) = X(z)(z^{-1} + \frac{1}{2})$$

$$\frac{1}{2}y_{t-1} + y_t = x_{t-1} + x_t$$

$$y_t = \frac{1}{2}x_t + x_{t-1} - \frac{1}{2}y_{t-1}$$

$$y_t = \frac{1}{2}x_t + x_{t-1} - \frac{1}{2}y_{t-1}$$

$$\textcircled{b} H(z) = \frac{z + z^{-1}}{2}$$

$$\textcircled{a} H(\omega) = \frac{1}{2}[\cos \omega + j \sin \omega + \cos \omega - j \sin \omega] = \cos \omega$$

$$|H(\omega)|^2 = \left[ \frac{1}{2}(\cos \omega + 1) \right]^2 + \left[ \frac{1}{2} \sin^2 \omega \right]^2$$

⑥ ①  $\frac{e^{j\omega/2} + 3e^{j\omega/2}}{e^{j\omega/2} + \frac{1}{3}e^{-j\omega/2}} \quad |H(\omega)|^2 = [20 \cdot \cos^2(\omega/2)]$

$\$ (20 \cos(\omega/2))^2 = 4 + 16$

$|H(\omega)| = \frac{(e^{j\omega/2} + 3e^{j\omega/2})^2}{(e^{j\omega/2} + \frac{1}{3}e^{-j\omega/2})^2} = \frac{3^2 (e^{j\omega/2} + e^{j\omega/2})^2}{(e^{j\omega/2} + \frac{1}{3}e^{-j\omega/2})^2}$

$\times q = \frac{\cos(\omega/2) - j \sin(\omega/2)}{\cos(\omega/2) + j \sin(\omega/2)}$

$e^{j\omega/2} + 3e^{j\omega/2} = e^{j\omega/2} + \frac{1}{3}e^{-j\omega/2}$   
 $3e^{j\omega/2} = \frac{1}{3}e^{-j\omega/2}$

$9e^{j\omega/2} = e^{-j\omega/2}$  ~~✗~~

②  $\frac{e^{j\omega/2} + 3e^{j\omega/2}}{e^{j\omega/2} - \frac{1}{3}}$

$e^{j\omega/2} - \frac{1}{3}e^{-j\omega/2} = e^{j\omega/2} + 3e^{j\omega/2}$

$-\frac{1}{3}e^{-j\omega/2} = 3e^{j\omega/2}$

$\times q = \frac{\cos(\omega/2) - j \sin(\omega/2)}{\cos(\omega/2) + j \sin(\omega/2)}$

③  $\frac{e^{j\omega/2} + 2e^{j\omega/2}}{e^{j\omega/2} + 2e^{-j\omega/2}}$

$2e^{-j\omega/2} = 2e^{j\omega/2}$

$\frac{2}{2} = \frac{e^{j\omega/2}}{e^{-j\omega/2}} = 1$  ✓

④  $\frac{e^{j\omega/2} - 2e^{j\omega/2}}{e^{j\omega/2} + 2e^{-j\omega/2}}$

$e^{j\omega/2} + 2e^{-j\omega/2} = e^{j\omega/2} - 2e^{j\omega/2}$

⑤

$\frac{1}{3} \cdot \frac{2 \cos^2(\omega)}{3} - \frac{2 \sin(\omega) \cos(\omega) j}{3}$

$$\boxed{7} \quad \begin{array}{l} x \approx 0 \\ x < 0 \end{array} \quad x = \tan(x) = \tan^{-1}(x)$$

$$\tan x = x + \frac{x^3}{3} + \frac{2x^5}{15} + \dots$$

$$\tan^{-1}(x) = x - \frac{x^3}{3} + \frac{x^5}{5} + \dots$$

Using 2<sup>nd</sup> order approximation:

$$\tan x = x + \frac{1}{3}x^3$$

$$x^3 < 0$$

$$\frac{1}{3}x^3 < 0$$

$$x + \frac{1}{3}x^3 < x$$

$$\therefore \tan x < x$$

$$\tan^{-1} x = x - \frac{1}{3}x^3$$

$$x^3 < 0$$

$$-\frac{1}{3}x^3 > 0$$

$$x - \frac{1}{3}x^3 > x$$

$$\therefore \tan^{-1} x > x$$

$$\tan x < x < \tan^{-1} x \quad (a)$$

$$\boxed{8} \quad L=9 \quad R=0.9$$

$$Y_t = X_t + 0.9^9 Y_{t-9} \quad H(z) = 1 + 0.387z^{-9}$$

$$\sum_{t=0}^{\infty} h_t$$

$$\delta_t = \{1, 0, 0, 0, 0, 0, \dots\}$$

$$h_0 = 1 \quad h_{9t} = [0.9^9]^t \quad \sum_{t=0}^{\infty} h_t = 1 +$$

$$\sum_{t=0}^{\infty} h_t = \frac{a}{1-r} \quad a=1 \quad r=0.387$$

$$\frac{1}{1-0.387} = 1.6313 \quad (c)$$